veric/initial_world.v
@@ -2,16 +2,20 @@ From iris.algebra Require Import csum agree.
 From iris_ora.algebra Require Import osum agree.
 Require Import VST.zlist.sublist.
 Require Import VST.veric.shared.
-Require Import VST.veric.resource_map.
 Require Import VST.veric.juicy_base.
 Require Import VST.veric.juicy_mem.
 Require Import VST.veric.juicy_mem_lemmas.
 (*Require Import VST.veric.juicy_mem_ops.*)
 Require Import VST.veric.res_predicates.
+Require Import VST.veric.resource_map.
 Require Import VST.veric.seplog.
 Require Import VST.veric.shares.
+Require Import VST.veric.dshare.
 Require Import VST.veric.mpred.
 Require Import VST.veric.mapsto_memory_block.
+Import Values.
+
+Open Scope maps.
 
 Lemma adr_range_divide:
   forall b i p q loc,
